src/Examples/DnsServer/DnsLemmas.v
@@ -13,6 +13,7 @@ Require Import
         Fiat.QueryStructure.Automation.SearchTerms.FindPrefixSearchTerms
         Fiat.QueryStructure.Automation.QSImplementation
         Fiat.Examples.DnsServer.Packet
+        Fiat.Examples.DnsServer.DecomposeSumField
         Fiat.Examples.DnsServer.AuthoritativeDNSSchema.
 
 Open Scope list_scope.
@@ -91,6 +92,64 @@ Proof.
   intros; refine pick val true; [ reflexivity | simpl; intros; assumption ].
 Qed.
 
+Lemma refine_forall_to_exists {A}
+  : forall (P Q : A -> Prop)
+           (R : @IndexedEnsemble A)
+           (P_dec : DecideableEnsemble P),
+    refine {b |
+            decides b
+                    (forall tup' : @IndexedElement A,
+                        R tup'
+                        -> Q (indexedElement tup')
+                        -> P (indexedElement tup'))}
+           (b <- {b |
+                  decides b
+                          (exists tup' : @IndexedElement A,
+                              R tup' /\
+                              Q (indexedElement tup')
+                              /\ ~ P (indexedElement tup'))};
+              ret (negb b)).
+Proof.
+  unfold refine; intros; computes_to_inv; subst.
+  destruct v0; simpl in *;
+    computes_to_econstructor; simpl; unfold not; intros.
+  - destruct_ex; intuition.
+  - destruct (dec (indexedElement tup')) eqn: ?.
+    rewrite dec_decides_P in Heqb; eauto.
+    rewrite Decides_false in Heqb.
+    elimtype False; eauto.
+Qed.
+
+Lemma refine_forall_to_exists_independent {A}
+  : forall n (P P' Q : A -> Prop) (R : @IndexedEnsemble A),
+    (P' n -> ~ P n)
+    -> P n
+    -> refine {b |
+               decides b
+                       (forall tup' : @IndexedElement A,
+                           R tup' ->
+                           Q (indexedElement tup') -> P' n)}
+              (b <- {b |
+                     decides b
+                             (exists tup' : @IndexedElement A,
+                                 R tup' /\
+                                 Q (indexedElement tup'))};
+                 ret (negb b)).
+Proof.
+  intros.
+  rewrite (@refine_forall_to_exists _ (fun _ => P' n)).
+  unfold refine; intros; computes_to_inv; subst.
+  refine pick val v0.
+  computes_to_econstructor; eauto.
+  destruct v0; simpl in *.
+  - destruct_ex; eexists; intuition eauto.
+  - intro; apply H1; destruct_ex; eexists; intuition eauto.
+  - eapply Build_DecideableEnsemble with (fun _ => false);
+      split; intros; eauto.
+    + discriminate.
+    + intuition.
+Qed.
+
 (* if the record's type *is* CNAME, then refine the forall check against other records into
 an existential (exists a record with the same name), and return the opposite *)
 Lemma refine_is_CNAME__forall_to_exists :
@@ -108,17 +167,15 @@ Lemma refine_is_CNAME__forall_to_exists :
                                  n!sNAME = (indexedElement tup')!sNAME)};
                  ret (negb b)).
 Proof.
-  repeat match goal with
-         | _ : _ ↝ _ |- _ => computes_to_inv
-         | _ : negb ?v = _ |- _ => destruct v; simpl in *; subst
-         | _ : ex _ |- _ => destruct_ex
-         | _ => progress first [ intro | computes_to_econstructor | simpl; intuition; eauto ]
-         end.
+  intros; eapply (@refine_forall_to_exists_independent
+                    _ n (fun n => RDataTypeToRRecordType (n!sRDATA) = CNAME)
+                    (fun n => RDataTypeToRRecordType (n!sRDATA) <> CNAME)
+                    (fun tup' => n!sNAME = tup'!sNAME) R); eauto.
 Qed.
 
 (* very similar to refine_is_CNAME__forall_to_exists;
 they start with the same set, but refine_forall_to_exists refines it with an extra end condition. changes the (forall x, ~P x) check into (exists x, P x) and returns !x, adding the condition in the forall *)
-Lemma refine_forall_to_exists :
+Lemma refine_forall_to_exists' :
   forall (n : resourceRecord) (R : @IndexedEnsemble resourceRecord),
     refine {b |
             decides b
@@ -151,6 +208,77 @@ unfold DomainName, Label;
   auto with typeclass_instances.
 Qed.
 
+Lemma UnConstrQuery_In_Where_Map {resultT}:
+  forall (qs_schema : RawQueryStructureSchema) (idx : Fin.t (numRawQSschemaSchemas qs_schema))
+         (r_o : UnConstrQueryStructure qs_schema) (P : Ensemble RawTuple)
+         (f : _ -> resultT),
+    refine (UnConstrQuery_In r_o idx (fun r : RawTuple => Where (P r)
+                                                                Return (f r)))
+           (results <- UnConstrQuery_In r_o idx (fun r : RawTuple => Where (P r)
+                                                                           Return r);
+              ret (map f results)).
+Proof.
+Admitted.
+
+Lemma Map_UnConstrQuery_In_Where {resultT}:
+  forall (qs_schema : RawQueryStructureSchema) (idx : Fin.t (numRawQSschemaSchemas qs_schema))
+         (r_o : UnConstrQueryStructure qs_schema) (P : Ensemble RawTuple)
+         (f : _ -> resultT),
+    refine (results <- UnConstrQuery_In r_o idx (fun r : RawTuple => Where (P r)
+                                                                           Return r);
+              ret (map f results))
+           (UnConstrQuery_In r_o idx (fun r : RawTuple => Where (P r)
+                                                                Return (f r))).
+Proof.
+Admitted.
+
+Lemma refine_under_bind_both_ambivalent {A A' B}
+  : forall (c : Comp A)
+           (c' : Comp A')
+           (x : A -> Comp B)
+           (y : A' -> Comp B),
+    (forall (a' : A'),
+        c' ↝ a' ->
+        exists a,
+          c ↝ a /\
+          refine (x a) (y a'))
+    -> refine (a <- c;
+                 x a)
+              (a <- c';
+                 y a).
+Proof.
+  unfold refine; intros; computes_to_inv.
+  apply H in H0; destruct_ex; intuition.
+  computes_to_econstructor; eauto.
+Qed.
+
+Corollary refine_Count_map :
+  forall (qs_schema : RawQueryStructureSchema) (idx : Fin.t (numRawQSschemaSchemas qs_schema))
+         (r_o : UnConstrQueryStructure qs_schema) (P : Ensemble RawTuple),
+    refine (Count For (UnConstrQuery_In r_o idx (fun r : RawTuple => Where (P r)
+                                                                           Return r)))
+           (Count For (UnConstrQuery_In r_o idx (fun r : RawTuple => Where (P r)
+                                                                           Return ()))).
+Proof.
+  Local Transparent Count.
+  Local Transparent Query_For.
+  unfold Count, Query_For; intros.
+  rewrite !refineEquiv_bind_bind.
+  eapply refine_under_bind_both_ambivalent; intros.
+  apply Map_UnConstrQuery_In_Where in H.
+  simpl in H; computes_to_inv; subst.
+  eexists; split; eauto.
+  eapply refine_under_bind_both_ambivalent; intros.
+  simpl in H; computes_to_inv; subst.
+  symmetry in H0.
+  eexists v; split; eauto.
+  apply Permutation_length in H0.
+  rewrite H0.
+  rewrite map_length; reflexivity.
+  Local Opaque Count.
+  Local Opaque Query_For.
+Qed.
+
 Lemma refine_count_constraint_broken :
   forall (n : resourceRecord) (r : UnConstrQueryStructure DnsSchema),
     refine {b |
@@ -162,7 +290,7 @@ Lemma refine_count_constraint_broken :
                Then count <- Count
                For (tup in r!sRRecords)
                (Where (n!sNAME = tup!sNAME)
-                      Return tup )%QueryImpl;
+                      Return () )%QueryImpl;
               ret (beq_nat count 0) Else ret true).
 Proof.
   (* intros; setoid_rewrite refine_pick_decides at 1. *)
@@ -200,7 +328,9 @@ Proof.
   intros; simplify with monad laws; simpl.
   autorewrite with monad laws.
   setoid_rewrite negb_involutive.
-  reflexivity.
+  apply refine_If_Then_Else; try reflexivity.
+  intros.
+  rewrite (@refine_Count_map DnsSchema Fin.F1); reflexivity.
 Qed.
 
 Hint Resolve refine_count_constraint_broken.
@@ -336,10 +466,10 @@ Lemma refine_count_constraint_broken' :
                                         (fun tup : Tuple =>
                                            Where (n!sNAME = tup!sNAME
                                                   /\ RDataTypeToRRecordType tup!sRDATA = CNAME ) (* extra /\ condition *)
-                                                 Return tup ));
+                                                 Return () ));
               ret (beq_nat count 0)).
 Proof.
-  intros; setoid_rewrite refine_forall_to_exists.
+  intros; setoid_rewrite refine_forall_to_exists'.
   (*refine existence check into query. *)
   match goal with
     |- context[{b | decides b
@@ -364,8 +494,9 @@ Proof.
   apply @DecideableEnsemble_And.  apply DecideableEnsemble_EqDec.
   auto with typeclass_instances.
   apply DecideableEnsemble_EqDec. apply Query_eq_RRecordType.
- simplify with monad laws.
+  simplify with monad laws.
   setoid_rewrite negb_involutive; f_equiv.
+  apply refine_Count_map.
 Qed.
 
 (* clear_nested_if, using filter_nil_is_nil, clear the nested if/then in honing AddData *)
@@ -586,174 +717,72 @@ Proof.
   destruct (IsPrefix_dec l1 l2); eauto.
 Qed.
 
+Lemma refine_For_List': forall (ResultT : Type) (bod : Comp (list ResultT)),
+    refine
+      (result <- bod;
+         {l : list ResultT | Permutation result l})
+      (For bod).
+Proof.
+  Local Transparent Query_For.
+  unfold Query_For; intros; reflexivity.
+  Local Opaque Query_For.
+Qed.
+
+Lemma flatten_CompList_Return' {A : Type}
+  : forall (l : list A),
+    refine (ret l) (FlattenCompList.flatten_CompList (map Query_Return l)).
+Proof.
+  induction l; simpl; try reflexivity.
+  unfold Query_Return at 1; rewrite refineEquiv_bind_unit.
+  setoid_rewrite <- IHl; rewrite refineEquiv_bind_unit.
+  simpl; reflexivity.
+Qed.
+
 (* Main lemma -- TODO generalize *)
 
-(* should be generalized *)
-Lemma tuples_in_relation_satisfy_constraint_specific :
-  forall (a : list RawTuple)
-         (n : packet)
-         (r_n : QueryStructure DnsSchema),
+Lemma tuples_in_relation_satisfy_constraint {qs_schema}:
+  forall (r_n : QueryStructure qs_schema)
+         Ridx P l (P_dec : DecideableEnsemble P),
     (* TODO *)
-    For (r in r_n!sRRecords)
-        (Where (prefix r!sNAME ((n!"question"!"qname" ))) (* Where Predicate ... *)
-               Return r ) ↝ a ->
-    forall (t t' : resourceRecord) (n0 n' : nat),
+    For (Query_In r_n Ridx
+                  (fun r => Where (P r) (* Where Predicate ... *)
+                                  Return r )) ↝ l ->
+    forall (t t' : _ ) (n0 n' : nat),
       n0 <> n' ->
-      nth_error a n0 = Some t -> (* this isn't right? *)
-      nth_error a n' = Some t' ->
-      get_name t = get_name t' ->
-      RDataTypeToRRecordType t!sRDATA <> CNAME.
+      nth_error l n0 = Some t -> (* this isn't right? *)
+      nth_error l n' = Some t' ->
+      SatisfiesTupleConstraints Ridx t t'.
 Proof.
-  intros. inversion H. inv H4.
-
-  assert (forall l,
-             In (list RawTuple)
-                (let qs_schema := DnsSchema in
-                 let r' := r_n in
-                 Query_In r' bCOLLECTIONS
-                          (fun r : RawTuple =>
-                             Return r )) l
-             ->  List.incl x l).
-  {
-    (* need to use the main H5 too, with the filter
-this is because x is a list of tuples that all came from r *)
-    clear t t' n0 H0 H1 H2 H3 H n'.
-    remember H5 as inFilter. clear HeqinFilter H5.
-    intros l inRelation.
-    inversion inFilter.
-    inv H.
-    simpl in *.
-
-    inv H0.
-    (* H : x0 (new) is x1 without indices, and all indices in x1 are unique, and
-     forall x2 (new) : indexedelement, it's in sRRecords if and only if it's in x1, the list of indexed elements  *)
-
-    inv H.
-    inv H2.
-    remember (map elementIndex x1) as x0.
-
-    inversion inRelation.
-    inversion H2. clear H2. inversion H3. clear H3.
-    inversion H2. clear H2. inversion H5. clear H5.
-    simpl in *.             (* TODO ltac for these inversions and reasoning about them *)
-
-    unfold incl.
-    subst. (* optional *)
-
-    intros filterElem filterH.
-    remember (map indexedElement x3) as x3elems.
-
-    assert (exists feIndex,
-               List.In {| elementIndex := feIndex; indexedElement := filterElem |} x1).
-    {
-      remember (map indexedElement x1) as x1elems.
-
-      (* this is the real nub of the proof *)
-      assert (List.incl x x1elems).
-      {
-        unfold incl.
-        intros xElem. intro.
-        match type of H1 with
-        | appcontext[map (fun r : @RawTuple ?H => (Where (@?H1 r) _))] =>
-          pose proof (In_flatten_CompList H1) as in_flatten
-        end.
-
-        assert ((exists a' : IndexedElement,
-                    List.In a' x1 /\ indexedElement a' = xElem) -> List.In xElem x1elems).
-        {
-          intros.
-          inversion H5. clear H5.
-          inversion H8. clear H8.
-          rewrite <- H9.
-          rewrite Heqx1elems.
-          apply in_map_iff.
-          eexists.
-          split.
-          reflexivity.
-          auto. }
-
-        apply H5. clear H5.
-
-        eapply in_flatten; eauto using string_dec.
-        intros; setoid_rewrite prefix_correct;
-          setoid_rewrite <- string_dec_bool_true_iff;
-          find_if_inside; eauto.
-
-        rewrite Heqx1elems in H1.
-        rewrite List.map_map in H1.
-        unfold In in H1.
-        apply H1.
-      }
-
-      unfold incl in H3.
-      specialize (H3 filterElem).
-
-      (* alternate version *)
-      assert (List.In filterElem x1elems ->
-              exists index, List.In {| elementIndex := index; indexedElement := filterElem |} x1).
-      {
-        intros.
-        rewrite Heqx1elems in H5.
-        apply in_map_iff in H5.
-        destruct H5.
-        destruct H5.
-
-        destruct x0.
-        simpl in *.
-        rewrite H5 in H8.
-        exists elementIndex.
-        apply H8. }
-
-      specialize (H3 filterH).
-      specialize (H5 H3).
-      destruct H5 as [index].
-      exists index.
-      apply H5.
-    }
-
-    (* ------------------------ *)
-
-    destruct H3 as [feIndex].                  (* new *)
-
-    remember (Build_IndexedElement feIndex filterElem) as indexedFilterElem.
-    specialize (H2 indexedFilterElem).
-    specialize (H indexedFilterElem).
-
-    inversion H. clear H.
-    inversion H2. clear H2.
-
-    specialize (H8 H3).
-    specialize (H H8).
-
-    clear H5 H8 H9.
-
-    eapply Permutation_in.
-    apply Permutation_sym.
-    apply flatmap_permutation; eauto.
-
-    (* there's probably something I can do with indices to remove this step *)
-    assert (List.In indexedFilterElem x3 -> List.In filterElem (map indexedElement x3)) as H5.
-    { intros.
-      apply in_map_iff.
-      exists indexedFilterElem.
-      split.
-      - rewrite HeqindexedFilterElem. reflexivity.
-      - auto. }
-
-    rewrite <- Heqx3elems in *.
-    apply H5. apply H.
-  }                              (* ends List.incl x l *)
+  intros.
+  apply refine_For_List' in H; computes_to_inv.
+  assert (forall l',
+             computes_to
+               (let qs_schema := DnsSchema in
+                let r' := r_n in
+                Query_In r' Ridx
+                         (fun r : RawTuple =>
+                            Return r )) l'
+             ->  List.incl l l').
+  { intros.
+    unfold Query_In, QueryResultComp, In in *; computes_to_inv.
+    unfold incl; intros.
+    apply flatten_CompList_Return' in H3'; computes_to_inv; subst.
+    pose proof (Permutation_UnIndexedEnsembleListEquivalence' H H3).
+    rewrite <- H5.
+    eapply flatten_CompList_Subset in H'0; eauto.
+    rewrite H'; assumption.
+  }
   (* ------------------------------------------------------------------------------------ *)
 
-  assert (Permutation a x) by (symmetry; apply H6).
+  assert (Permutation l v) by (symmetry; apply H').
 
   (* prove that everything in a is in sRRecords *)
-  assert (forall l,
+  assert (forall l',
              In (list RawTuple)
                 (let qs_schema := DnsSchema in
                  let r' := r_n in
-                 Query_In r' bCOLLECTIONS (fun r : RawTuple => Return r)) l ->
-             incl a l).
+                 Query_In r' Ridx (fun r : RawTuple => Return r)) l' ->
+             incl l l').
   {
     (* x \subset sRRecords, and Permutation a x *)
     intros allTuplesInRelation inRelation.
@@ -762,69 +791,82 @@ this is because x is a list of tuples that all came from r *)
     intros aTuple inA.
     unfold incl in H4.
 
-    clear H H5. clear t t' n0 n' H0 H1 H2 H3.
-
-    specialize (H4 allTuplesInRelation inRelation aTuple).
-    apply H4.
-    eapply Permutation_in.
-    apply H7. auto.
+    eapply (H3 allTuplesInRelation inRelation aTuple); eauto.
   }
 
   (* use the proof that the constraints hold on everything in sC, therefore on a *)
   (* t and t' are in a, therefore the constraint must hold on them *)
   (* this is the top-level goal  *)
 
-  assert (List.In t a).
+  assert (List.In t l).
   { apply exists_in_list. exists n0. auto. }
-  assert (List.In t' a).
+  assert (List.In t' l).
   { apply exists_in_list. exists n'. auto. }
 
-  assert (List.In t x).
-  { eapply Permutation_in. apply H7. auto. }
-  assert (List.In t' x).
-  { eapply Permutation_in. apply H7. auto. }
   simpl in H5.
-  eapply refine_Intersection_Where in H5.
-  unfold QueryResultComp in H5; computes_to_inv.
-  destruct H5 as [x' [Equiv [Equiv' Equiv''] ] ].
+  eapply refine_Intersection_Where in H.
+  unfold QueryResultComp in H; computes_to_inv.
+  destruct H as [x' [Equiv [Equiv' Equiv''] ] ].
   rewrite <- Equiv in *.
-  eapply flatmap_permutation in H5'; rewrite H5' in H7.
-  destruct (unindexed_OK_exists_index' _ H0 H1 H2 H7) as [m [m' [idx [idx' ?] ] ] ];
+  eapply flatmap_permutation in H'0; rewrite H'0 in H4.
+  destruct (unindexed_OK_exists_index' _ H0 H1 H2 H4) as [m [m' [idx [idx' ?] ] ] ];
     intuition.
 
-  pose proof (rawTupleconstr (ith2 (rawRels r_n) (Fin.F1 ))) as
+  pose proof (rawTupleconstr (ith2 (rawRels r_n) (Ridx ))) as
       constraint_in_relation_OK; simpl in *.
-  apply (constraint_in_relation_OK {| elementIndex := idx; indexedElement := t |}
-                                   {| elementIndex := idx'; indexedElement := t' |});
+  unfold GetNRelSchema.
+  destruct (tupleConstraints (Vector.map schemaRaw (QSschemaSchemas qs_schema))[@Ridx]); eauto;
+    apply (constraint_in_relation_OK {| elementIndex := idx; indexedElement := t |}
+                                     {| elementIndex := idx'; indexedElement := t' |});
     simpl; try eassumption.
 
-  eapply map_nth_error with (f := elementIndex) in H5.
-  eapply map_nth_error with (f := elementIndex) in H16.
+  eapply map_nth_error with (f := elementIndex) in H.
+  eapply map_nth_error with (f := elementIndex) in H10.
   {
-    revert m m' H5 H16 H14 Equiv''; clear; unfold Tuple; simpl; induction (map elementIndex x').
+    revert m m' H H10 H8 Equiv''; clear; unfold Tuple; simpl; induction (map elementIndex x').
     - destruct m; destruct m'; simpl; intros; try discriminate.
     - destruct m; destruct m'; simpl; intros; try discriminate.
       + intuition.
       + inversion Equiv''; subst.
-        intro; subst; apply H1; injections; apply exists_in_list; eauto.
+        intro; subst; apply H2; injections; apply exists_in_list; eauto.
       + inversion Equiv''; subst.
-        intro; subst; apply H1; injections; apply exists_in_list; eauto.
+        intro; subst; apply H2; injections; apply exists_in_list; eauto.
       + inversion Equiv''; eauto.
   }
 
   assert (List.In {| elementIndex := idx; indexedElement := t |} x').
   { eapply exists_in_list; eauto. }
-  apply Equiv' in H15; destruct H15; apply H15.
+  apply Equiv' in H9; destruct H9; apply H9.
   assert (List.In {| elementIndex := idx'; indexedElement := t' |} x').
   { eapply exists_in_list; eauto. }
-  apply Equiv' in H15; destruct H15;  apply H15.
+  apply Equiv' in H9; destruct H9;  apply H9.
+  eauto.
+Qed.
+
+Lemma tuples_in_relation_satisfy_constraint_specific :
+  forall (a : list RawTuple)
+         name
+         (r_n : QueryStructure DnsSchema),
+    For (r in r_n!sRRecords)
+        (Where (prefix r!sNAME name) (* Where Predicate ... *)
+               Return r ) ↝ a ->
+    forall (t t' : resourceRecord) (n0 n' : nat),
+      n0 <> n' ->
+      nth_error a n0 = Some t -> (* this isn't right? *)
+      nth_error a n' = Some t' ->
+      get_name t = get_name t' ->
+      RDataTypeToRRecordType t!sRDATA <> CNAME.
+Proof.
+  intros.
+  eapply (@tuples_in_relation_satisfy_constraint DnsSchema) in H; try eassumption.
+  simpl in *; intuition.
   apply DecideableEnsemble_bool.
 Qed.
 
-Lemma refine_beq_RRecordType_dec :
-  forall rr : resourceRecord,
-    refine {b | decides b (RDataTypeToRRecordType rr!sRDATA = CNAME)}
-           (ret (beq_RRecordType (RDataTypeToRRecordType rr!sRDATA) CNAME)).
+Lemma refine_beq_RRecordType_dec v :
+  forall (rr : resourceRecord),
+    refine {b | decides b (RDataTypeToRRecordType rr!sRDATA = v)}
+           (ret (beq_RRecordType (RDataTypeToRRecordType rr!sRDATA) v)).
 Proof.
   intros; rewrite <- beq_RRecordType_dec.
   intros; refine pick val _.
@@ -835,58 +877,263 @@ Qed.
 Lemma refine_noDup_CNAME_check :
   forall (rr : resourceRecord)
          (R : @IndexedEnsemble resourceRecord),
-  (forall tup tup' : IndexedElement,
-          elementIndex tup <> elementIndex tup' ->
-          R tup ->
-          R tup' ->
-          (indexedElement tup)!sNAME = (indexedElement tup')!sNAME
-          -> RDataTypeToRRecordType (indexedElement tup)!sRDATA <> CNAME)
-  -> refine {b |
-            decides b
-                    (forall tup',
-                        R tup' ->
-                        rr!sNAME = (indexedElement tup')!sNAME -> RDataTypeToRRecordType rr!sRDATA <> CNAME)}
-           (If (beq_RRecordType (RDataTypeToRRecordType rr!sRDATA) CNAME)
-               Then count <- Count
-               For
-               (QueryResultComp R
-                                (fun tup => Where (rr!sNAME = tup!sNAME)
-                                                  Return tup )%QueryImpl);
-                  ret (beq_nat count 0) Else ret true).
+    (forall tup tup' : IndexedElement,
+        elementIndex tup <> elementIndex tup' ->
+        R tup ->
+        R tup' ->
+        (indexedElement tup)!sNAME = (indexedElement tup')!sNAME
+        -> RDataTypeToRRecordType (indexedElement tup)!sRDATA <> CNAME)
+    -> refine {b |
+               decides b
+                       (forall tup',
+                           R tup' ->
+                           rr!sNAME = (indexedElement tup')!sNAME -> RDataTypeToRRecordType rr!sRDATA <> CNAME)}
+              (If (beq_RRecordType (RDataTypeToRRecordType rr!sRDATA) CNAME)
+                  Then count <- Count
+                  For
+                  (QueryResultComp R
+                                   (fun tup => Where (rr!sNAME = tup!sNAME)
+                                                     Return tup )%QueryImpl);
+                 ret (beq_nat count 0) Else ret true).
 Proof.
   intros.
-    intros; setoid_rewrite refine_pick_decides at 1;
+  intros; setoid_rewrite refine_pick_decides at 1;
     [ | apply refine_is_CNAME__forall_to_exists | apply refine_not_CNAME__independent ].
-    setoid_rewrite refine_beq_RRecordType_dec; simplify with monad laws.
-    apply refine_If_Then_Else; eauto.
-    setoid_rewrite refine_constraint_check_into_QueryResultComp with (P := fun tup => rr!sNAME = tup!sNAME).
-    rewrite refineEquiv_bind_bind.
-    f_equiv.
-    unfold pointwise_relation; intros; simplify with monad laws;
-      rewrite <- negb_involutive_reverse; reflexivity.
-    auto with typeclass_instances.
-    intuition.
-    reflexivity.
+  setoid_rewrite refine_beq_RRecordType_dec; simplify with monad laws.
+  apply refine_If_Then_Else; eauto.
+  setoid_rewrite refine_constraint_check_into_QueryResultComp with (P := fun tup => rr!sNAME = tup!sNAME).
+  rewrite refineEquiv_bind_bind.
+  f_equiv.
+  unfold pointwise_relation; intros; simplify with monad laws;
+    rewrite <- negb_involutive_reverse; reflexivity.
+  auto with typeclass_instances.
+  intuition.
+  reflexivity.
 Qed.
 
 Corollary refine_noDup_CNAME_check_dns :
   forall (rr : resourceRecord) r_o r_n,
     @DropQSConstraints_AbsR DnsSchema r_o r_n
-  -> refine {b |
-            decides b
-                    (forall tup',
-                        (GetUnConstrRelation r_n Fin.F1) tup' ->
-                        rr!sNAME = (indexedElement tup')!sNAME -> (RDataTypeToRRecordType rr!sRDATA) <> CNAME)}
-           (If (beq_RRecordType (RDataTypeToRRecordType rr!sRDATA) CNAME)
-               Then count <- Count
-               For
-               (UnConstrQuery_In r_n Fin.F1
-                                (fun tup => Where (rr!sNAME = tup!sNAME)
-                                                  Return tup )%QueryImpl);
-                  ret (beq_nat count 0) Else ret true).
+    -> refine {b |
+               decides b
+                       (forall tup',
+                           (GetUnConstrRelation r_n Fin.F1) tup' ->
+                           rr!sNAME = (indexedElement tup')!sNAME -> (RDataTypeToRRecordType rr!sRDATA) <> CNAME)}
+              (If (beq_RRecordType (RDataTypeToRRecordType rr!sRDATA) CNAME)
+                  Then count <- Count
+                  For
+                  (UnConstrQuery_In r_n Fin.F1
+                                    (fun tup => Where (rr!sNAME = tup!sNAME)
+                                                      Return () )%QueryImpl);
+                 ret (beq_nat count 0) Else ret true).
 Proof.
-  intros; eapply refine_noDup_CNAME_check.
+  intros; rewrite refine_noDup_CNAME_check.
+  setoid_rewrite (@refine_Count_map DnsSchema Fin.F1 r_n); reflexivity.
   intros; eapply (DropQSConstraints_AbsR_SatisfiesTupleConstraints H Fin.F1); eauto.
+Qed.
+
+Lemma refine_decides_Equiv_Ensemble' {A}:
+  forall (P P' : Ensemble A),
+    ((forall idx : A, P idx) <-> (forall idx' : A, P' idx')) ->
+    refine {b : bool | decides b (forall idx : A, P idx)} {b : bool | decides b (forall idx : A, P' idx)}.
+Proof.
+  intros; eapply refineEquiv_pick_pick.
+  intro; destruct x; simpl; split; intros; intuition eauto.
+Qed.
+
+Lemma refine_no_usurp_authority_check :
+  forall (rr : resourceRecord)
+         (R : @IndexedEnsemble resourceRecord),
+    (forall tup tup' : IndexedElement,
+        elementIndex tup <> elementIndex tup' ->
+        R tup ->
+        R tup' ->
+        (indexedElement tup)!sNAME = (indexedElement tup')!sNAME
+        -> RDataTypeToRRecordType (indexedElement tup)!sRDATA = NS
+        -> RDataTypeToRRecordType (indexedElement tup')!sRDATA <> NS
+        -> prefix (indexedElement tup)!sNAME (indexedElement tup')!sNAME
+        -> (indexedElement tup)!sNAME = (indexedElement tup')!sNAME)
+    -> refine {b |
+               decides b
+                       (forall tup',
+                           R tup'
+                           -> RDataTypeToRRecordType rr!sRDATA = NS
+                           -> RDataTypeToRRecordType (indexedElement tup')!sRDATA <> NS
+                           -> prefix rr!sNAME (indexedElement tup')!sNAME
+                           -> rr!sNAME = (indexedElement tup')!sNAME)}
+              (If (beq_RRecordType (RDataTypeToRRecordType rr!sRDATA) NS)
+                  Then count <- Count
+                  For
+                  (QueryResultComp R
+                                   (fun tup => Where (rr!sNAME <> tup!sNAME
+                                                      /\ RDataTypeToRRecordType tup!sRDATA <> NS
+                                                      /\ prefix (rr!sNAME) (tup!sNAME))
+                                                     Return tup )%QueryImpl);
+                 ret (beq_nat count 0) Else ret true).
+Proof.
+  intros.
+  let p := constr:(RDataTypeToRRecordType (rr!sRDATA : RDataType) = NS) in
+  intros; setoid_rewrite refine_pick_decides with (P := p) at 1.
+  setoid_rewrite refine_beq_RRecordType_dec; simplify with monad laws.
+  finish honing.
+  { intros.
+    erewrite refine_decides_Equiv_Ensemble' with (P' := fun tup' => R tup' ->
+                                                                    (_ (indexedElement tup') /\
+                                                                     _ (indexedElement tup'))
+                                                                    -> rr!sNAME = (indexedElement tup')!sNAME).
+    Focus 2.
+    split; intros.
+    apply H1.
+    eassumption.
+    eassumption.
+    pattern (indexedElement idx'). apply (proj1 H3).
+    pattern (indexedElement idx'). apply (proj2 H3).
+    eauto.
+    pose proof (@refine_forall_to_exists _
+                                         (fun idx => rr!sNAME = idx!sNAME)
+                                         (fun tup =>
+                                            (fun r : resourceRecord => RDataTypeToRRecordType r!sRDATA <> NS /\
+                                                                       is_true (prefix rr!sNAME r!sNAME)) tup)
+                                         R _);  simpl in *; erewrite H1.
+    setoid_rewrite refine_constraint_check_into_QueryResultComp.
+    simplify with monad laws.
+    setoid_rewrite <- negb_involutive_reverse.
+    finish honing.
+    apply DecideableEnsemble_And.
+    unfold Same_set, Included, In; intuition.
+  }
+  intros; refine pick val _.
+  finish honing.
+  simpl; intros; intuition.
+Qed.
+
+Corollary refine_no_usurp_authority_check_dns :
+  forall (rr : resourceRecord) r_o r_n,
+    @DropQSConstraints_AbsR DnsSchema r_o r_n
+    -> refine {b |
+               decides b
+                       (forall tup',
+                           (GetUnConstrRelation r_n Fin.F1) tup'
+                           -> RDataTypeToRRecordType rr!sRDATA = NS
+                           -> RDataTypeToRRecordType (indexedElement tup')!sRDATA <> NS
+                           -> prefix rr!sNAME (indexedElement tup')!sNAME
+                           -> rr!sNAME = (indexedElement tup')!sNAME)}
+              (If (beq_RRecordType (RDataTypeToRRecordType rr!sRDATA) NS)
+                  Then count <- Count
+                  For (UnConstrQuery_In r_n Fin.F1
+                                        (fun tup => Where (rr!sNAME <> tup!sNAME
+                                                           /\ RDataTypeToRRecordType tup!sRDATA <> NS
+                                                           /\ prefix (rr!sNAME) (tup!sNAME))
+                                                          Return () )%QueryImpl);
+                 ret (beq_nat count 0) Else ret true).
+Proof.
+  intros; rewrite refine_no_usurp_authority_check.
+  setoid_rewrite (@refine_Count_map DnsSchema Fin.F1 r_n); reflexivity.
+  intros; eapply (DropQSConstraints_AbsR_SatisfiesTupleConstraints H Fin.F1); eauto.
+Qed.
+
+Lemma refine_no_usurp_authority_check' :
+  forall (rr : resourceRecord)
+         (R : @IndexedEnsemble resourceRecord),
+    (forall tup tup' : IndexedElement,
+        elementIndex tup <> elementIndex tup' ->
+        R tup ->
+        R tup' ->
+        (indexedElement tup)!sNAME = (indexedElement tup')!sNAME
+        -> RDataTypeToRRecordType (indexedElement tup)!sRDATA = NS
+        -> RDataTypeToRRecordType (indexedElement tup')!sRDATA <> NS
+        -> prefix (indexedElement tup)!sNAME (indexedElement tup')!sNAME
+        -> (indexedElement tup)!sNAME = (indexedElement tup')!sNAME)
+    -> refine {b |
+               decides b
+                       (forall tup' : IndexedElement,
+                           R tup' ->
+                           RDataTypeToRRecordType (indexedElement tup')!sRDATA = NS ->
+                           RDataTypeToRRecordType rr!sRDATA <> NS ->
+                           prefix (indexedElement tup')!sNAME rr!sNAME -> (indexedElement tup')!sNAME = rr!sNAME)}
+              (If (beq_RRecordType (RDataTypeToRRecordType rr!sRDATA) NS) Then
+                  (ret true)
+                  Else
+                  (count <- Count
+                         For
+                         (QueryResultComp R
+                                          (fun tup => Where (RDataTypeToRRecordType tup!sRDATA = NS
+                                                             /\ prefix (tup!sNAME) (rr!sNAME)
+                                                             /\ tup!sNAME <> rr!sNAME)
+                                                            Return tup )%QueryImpl);
+                     ret (beq_nat count 0))).
+Proof.
+  intros.
+  let p := constr:(RDataTypeToRRecordType (rr!sRDATA : RDataType) = NS) in
+  intros; setoid_rewrite refine_pick_decides with (P := p) at 1.
+  setoid_rewrite refine_beq_RRecordType_dec; simplify with monad laws.
+  finish honing.
+  - intros; refine pick val _.
+    finish honing.
+    simpl; intros; intuition.
+  - intros.
+    erewrite refine_decides_Equiv_Ensemble' with (P' := fun tup' => R tup' ->
+                                                                    (_ (indexedElement tup') /\
+                                                                     _ (indexedElement tup'))
+                                                                    -> (indexedElement tup')!sNAME = rr!sNAME).
+    Focus 2.
+    split; intros.
+    apply H1.
+    eassumption.
+    pattern (indexedElement idx'). apply (proj1 H3).
+    eassumption.
+    pattern (indexedElement idx'). apply (proj2 H3).
+    eauto.
+    pose proof (@refine_forall_to_exists _
+                                         (fun idx => idx!sNAME = rr!sNAME)
+                                         (fun tup =>
+                                            (fun r : resourceRecord =>
+                                               RDataTypeToRRecordType r!sRDATA = NS
+                                               /\ is_true (prefix r!sNAME rr!sNAME )) tup)
+                                         R _);  simpl in *; erewrite H1.
+    setoid_rewrite refine_constraint_check_into_QueryResultComp.
+    simplify with monad laws.
+    setoid_rewrite <- negb_involutive_reverse.
+    finish honing.
+    apply DecideableEnsemble_And.
+    unfold Same_set, Included, In; intuition.
+Qed.
+
+Corollary refine_no_usurp_authority_check'_dns :
+  forall (rr : resourceRecord) r_o r_n,
+    @DropQSConstraints_AbsR DnsSchema r_o r_n
+    ->
+    refine {b |
+            decides b
+                    (forall tup' : IndexedElement,
+                        (GetUnConstrRelation r_n Fin.F1) tup' ->
+                        RDataTypeToRRecordType (indexedElement tup')!sRDATA = NS ->
+                        RDataTypeToRRecordType rr!sRDATA <> NS ->
+                        prefix (indexedElement tup')!sNAME rr!sNAME -> (indexedElement tup')!sNAME = rr!sNAME)}
+           (If (beq_RRecordType (RDataTypeToRRecordType rr!sRDATA) NS) Then
+               (ret true)
+               Else
+               (count <- Count
+                      For
+                      (UnConstrQuery_In r_n Fin.F1
+                                        (fun tup => Where (RDataTypeToRRecordType tup!sRDATA = NS
+                                                           /\ prefix (tup!sNAME) (rr!sNAME)
+                                                           /\ tup!sNAME <> rr!sNAME)
+                                                          Return () )%QueryImpl);
+                  ret (beq_nat count 0))).
+Proof.
+  intros; rewrite refine_no_usurp_authority_check'.
+  setoid_rewrite (@refine_Count_map DnsSchema Fin.F1 r_n); reflexivity.
+  intros; eapply (DropQSConstraints_AbsR_SatisfiesTupleConstraints H Fin.F1); eauto.
+Qed.
+
+Lemma beq_RRecordType_trans
+  : forall RType RType' RType'' ,
+    beq_RRecordType RType RType' = true
+    -> beq_RRecordType RType RType'' = beq_RRecordType RType'' RType'.
+Proof.
+  unfold beq_RRecordType; intros.
+  rewrite fin_beq_dec in H; subst; apply beq_RRecordType_sym.
 Qed.
 
 Instance ADomainName_eq : Query_eq DomainName := Astring_eq.
@@ -949,7 +1196,7 @@ Proof.
     assert (exists v',
                computes_to
                  (FlattenCompList.flatten_CompList (map (fun a : A => Where (op (f a) bound)
-                                                                         Return a ) v0)) v').
+                                                                            Return a ) v0)) v').
     {
       revert op_dec; clear; induction v0; simpl; intros; eauto.
       destruct IHv0; eauto.
@@ -1044,30 +1291,13 @@ Proof.
         apply H2 in n; subst; eauto.
 Qed.
 
-Lemma refine_under_bind_both_ambivalent {A B}
-  : forall (c c' : Comp A)
-           (x y : A -> Comp B),
-    (forall (a' : A),
-        c' ↝ a' ->
-        exists a,
-          c ↝ a /\
-          refine (x a) (y a'))
-    -> refine (a <- c;
-                 x a)
-              (a <- c';
-                 y a).
-Proof.
-  unfold refine; intros; computes_to_inv.
-  apply H in H0; destruct_ex; intuition.
-  computes_to_econstructor; eauto.
-Qed.
 
 Local Transparent Query_For.
 
 Lemma refine_MaxElements_For {A}
   : forall (op : A -> A -> Prop) ens,
     refine (MaxElements op For ens)
-        (MaxElements op ens).
+           (MaxElements op ens).
 Proof.
   unfold MaxElements; intros.
   rewrite refine_For.
@@ -1081,15 +1311,15 @@ Lemma MaxElementsUnConstrQuery_In {qs_schema}
   : forall idx f bound (r_o : UnConstrQueryStructure qs_schema),
     refine (MaxElements (fun r r' : RawTuple => prefix (f r) (f r'))
                         For (UnConstrQuery_In r_o idx (fun r : RawTuple => Where (prefix (f r) bound)
-                                                                         Return r )))
+                                                                                 Return r )))
            (results' <- For (UnConstrQuery_In r_o idx (fun r : RawTuple => Where (f r = bound)
-                                                                         Return r ));
+                                                                                 Return r ));
               If negb (is_empty results') Then ret results' Else
                  (MaxElements (fun r r' => prefix (f r) (f r'))
                               For (UnConstrQuery_In r_o idx (fun r : RawTuple => Where (prefix (f r) bound
-                                                                                /\ (f r) <> bound)
-                                                                         Return r )))
-).
+                                                                                        /\ (f r) <> bound)
+                                                                                       Return r )))
+           ).
 Proof.
   intros.
   pose proof (fun H H' H'' H''' =>
@@ -1132,6 +1362,507 @@ Proof.
   Local Opaque QueryResultComp. *)
 Admitted.
 
+Lemma refine_Process_Query
+  : forall (r_o : QueryStructure DnsSchema)
+           (r_n : UnConstrQueryStructure DnsSchema)
+           bound,
+    DropQSConstraints_AbsR r_o r_n
+    -> refine (For (UnConstrQuery_In r_n Fin.F1
+                                     (fun r : RawTuple => Where (GetAttributeRaw r Fin.F1 = bound)
+                                                                Return r )))
+              (results <- For (UnConstrQuery_In r_n Fin.F1
+                                                (fun r : RawTuple => Where
+                                                                       ((RDataTypeToRRecordType r!sRDATA) = CNAME
+                                                                        /\ GetAttributeRaw r Fin.F1 = bound)
+                                                                       Return r ));
+                 (Ifopt (hd_error results) as record Then
+                                                     (ret [record])
+                                                     Else
+                                                     For (UnConstrQuery_In r_n Fin.F1
+                                                                           (fun r : RawTuple => Where
+                                                                                                  ((RDataTypeToRRecordType r!sRDATA) <> CNAME
+                                                                                                   /\ GetAttributeRaw r Fin.F1 = bound)
+                                                                                                  Return r )))).
+Proof.
+  unfold refine; intros.
+  computes_to_inv.
+  destruct v0; simpl in *; eauto.
+  - admit.
+  - computes_to_inv; subst.
+    Local Transparent Query_For.
+    Local Transparent QueryResultComp.
+    unfold UnConstrQuery_In, Query_For, QueryResultComp in *; computes_to_inv.
+    apply refineEquiv_bind_bind.
+    computes_to_econstructor; eauto; clear H0.
+    revert v v0 H0'0 H0'.
+    induction v1; simpl in *; intros.
+    + computes_to_inv; subst.
+      apply Permutation_nil in H0'; discriminate.
+    + unfold Query_Where at 1, Query_Return at 1 in H0'0.
+      computes_to_inv; subst.
+      intuition.
+      apply refineEquiv_bind_bind.
+      match goal with
+        |- context [GetAttributeRaw ?a ?idx] =>
+        destruct (string_dec (GetAttributeRaw a idx) bound)
+      end.
+      * computes_to_econstructor.
+        computes_to_econstructor.
+        split; intros.
+        computes_to_econstructor.
+        congruence.
+        unfold GetAttribute in *; simpl in *.
+        destruct ((RDataTypeToRRecordType (GetAttributeRaw a (Fin.FS (Fin.FS (Fin.FS Fin.F1))))) == CNAME).
+        { apply H2 in e0; eauto.
+          computes_to_inv; subst.
+Admitted.
+
+(*       apply refineEquiv_bind_bind. *)
+(*       computes_to_econstructor. *)
+
+(*       setoid_rewrite refine_Query_Where_False_Cond. *)
+(*       rewrite refine_QueryResultComp_body_Where_False      . *)
+
+
+
+(*       inversion H0'. *)
+(*     computes_to_econstructor. *)
+(*     computes_to_econstructor. *)
+(*     computes_to_inv; subst; computes_to_econstructor; split; intros. *)
+(*       discriminate. *)
+(*       intuition. *)
+(*     + match goal with *)
+(*         H : context[fin_eq_dec ?X ?Y] |- _ => *)
+(*         destruct (fin_eq_dec X Y); simpl in H *)
+(*       end. *)
+(*       * computes_to_inv; subst. *)
+(*         destruct l; simpl in *. *)
+(*         { computes_to_econstructor; split; intros. *)
+(*           injections. *)
+(*           split; eauto; left. *)
+(*           destruct b as [? [? [? [? ?] ] ] ]; simpl in *. *)
+(*           unfold Tuple_DecomposeRawQueryStructure_inj'; simpl. *)
+(*           unfold icons2, ilist2_hd, ilist2_tl; simpl; repeat f_equal. *)
+(*           unfold SumType.inj_SumType; simpl. *)
+(*           unfold CNAME_Record2RRecord; simpl. *)
+(*           unfold VariantResourceRecord2RRecord; simpl. *)
+(*           unfold icons2; simpl. *)
+(*           repeat f_equal. *)
+(*           unfold Domain; simpl; reflexivity. *)
+(*           unfold Domain; simpl; reflexivity. *)
+(*           destruct prim_snd; destruct (@inil2 Type); reflexivity. *)
+(*           f_equal. *)
+(*           intuition. *)
+(*           destruct b as [? [? [? [? ?] ] ] ]; simpl in *. *)
+(*           unfold Tuple_DecomposeRawQueryStructure_inj' in *; simpl in *. *)
+(*           unfold icons2, ilist2_hd, ilist2_tl in *; simpl in *; *)
+(*             unfold SumType.inj_SumType in *; simpl in *. *)
+(*           unfold CNAME_Record2RRecord in *; simpl in *. *)
+(*           unfold VariantResourceRecord2RRecord in *; simpl in *. *)
+(*           unfold icons2 in *; simpl in *. *)
+(*           destruct v0 as [? [? [? [? ?] ] ] ]; simpl in *. *)
+(*           injections; simpl. *)
+(*           repeat f_equal. *)
+(*           destruct prim_snd; destruct (@inil2 Type); reflexivity. *)
+(*         } *)
+(*         admit. *)
+(*       * admit. *)
+(* Admitted. *)
+
+Lemma is_empty_app {A} : forall l1 l2 : list A,
+    is_empty (l1 ++ l2) = is_empty l1 && is_empty l2.
+Proof.
+  induction l1; simpl; eauto.
+Qed.
+
+Lemma negb_is_empty_app {A} : forall l1 l2 : list A,
+    negb (is_empty (l1 ++ l2)) = negb (is_empty l1) || negb (is_empty l2).
+Proof.
+  intros; rewrite is_empty_app.
+  rewrite negb_andb; reflexivity.
+Qed.
+
+Lemma eq_If_orb {A}
+  : forall i1 i2 (t e : A) ,
+    If i1 || i2 Then t Else e =
+    If i1 Then t Else
+       (If i2 Then t Else e).
+Proof.
+  intros; destruct i1; simpl; eauto.
+Qed.
+
+Arguments SumType.inj_SumType : simpl never.
+
+Lemma refine_Singleton_Set
+  : forall (r_n : UnConstrQueryStructure DnsSchema) q bound a,
+    For (UnConstrQuery_In r_n Fin.F1
+                          (fun r : RawTuple =>
+                             Where (RDataTypeToRRecordType r!sRDATA = CNAME /\ GetAttributeRaw r Fin.F1 = bound)
+                                   Return r )) ↝ [a]
+    -> refine
+         (SingletonSet (fun b : CNAME_Record =>
+                          List.In (A := resourceRecord) b [a]
+                          /\ q <> QType_inj CNAME))
+         (If q == (QType_inj CNAME) Then
+                                    (ret None)
+                                    Else
+                                    (c_record <- {c_record : CNAME_Record | a =
+                                                                            @Tuple_DecomposeRawQueryStructure_inj'
+                                                                              _ DnsSchema Fin.F1 (Fin.FS (Fin.FS (Fin.FS (Fin.F1)))) _
+                                                                              (SumType.inj_SumType ResourceRecordTypeTypes)
+                                                                              CNAME c_record  };
+                                       ret (Some c_record))).
+Proof.
+  unfold refine; intros.
+  destruct (q == CNAME); simpl in *; computes_to_inv; subst.
+  - computes_to_econstructor; split; intros.
+    discriminate.
+    intuition.
+  - unfold SingletonSet.
+    computes_to_econstructor; split; intros.
+    + pose proof (@For_UnConstrQuery_In_Where_Prop DnsSchema Fin.F1 r_n _ _ _ H);
+        inversion H1; subst; eauto.
+      injection H0; intro; subst.
+      intuition.
+      left.
+      destruct b as [? [? [? [? ?] ] ] ]; simpl in *.
+      unfold Tuple_DecomposeRawQueryStructure_inj'; simpl.
+      unfold icons2, ilist2_hd, ilist2_tl; simpl; repeat f_equal.
+      unfold SumType.inj_SumType; simpl.
+      unfold CNAME_Record2RRecord; simpl.
+      unfold VariantResourceRecord2RRecord; simpl.
+      unfold icons2; simpl.
+      destruct prim_snd; destruct (@inil2 Type); reflexivity.
+    + f_equal.
+      intuition.
+      destruct b as [? [? [? [? ?] ] ] ]; simpl in *.
+      unfold Tuple_DecomposeRawQueryStructure_inj' in *; simpl in *.
+      unfold icons2, ilist2_hd, ilist2_tl in *; simpl in *;
+        unfold SumType.inj_SumType in *; simpl in *.
+      unfold CNAME_Record2RRecord in *; simpl in *.
+      unfold VariantResourceRecord2RRecord in *; simpl in *.
+      unfold icons2 in *; simpl in *.
+      destruct v0 as [? [? [? [? ?] ] ] ]; simpl in *.
+      injections; simpl.
+      destruct prim_snd; destruct (@inil2 Type); reflexivity.
+Qed.
+
+Lemma refine_Singleton_Set''
+  : forall (r_o : QueryStructure DnsSchema)
+           (r_n : UnConstrQueryStructure DnsSchema) q bound l a,
+    For (UnConstrQuery_In r_n Fin.F1
+                          (fun r : RawTuple =>
+                             Where (RDataTypeToRRecordType r!sRDATA = CNAME /\ GetAttributeRaw r Fin.F1 = bound)
+                                   Return r )) ↝ l
+    -> hd_error l = Some a
+    -> refine
+         (SingletonSet (fun b : CNAME_Record =>
+                          List.In (A := resourceRecord) b [a]
+                          /\ q <> QType_inj CNAME))
+         (If q == (QType_inj CNAME) Then
+                                    (ret None)
+                                    Else
+                                    (c_record <- {c_record : CNAME_Record | a =
+                                                                            @Tuple_DecomposeRawQueryStructure_inj'
+                                                                              _ DnsSchema Fin.F1 (Fin.FS (Fin.FS (Fin.FS (Fin.F1)))) _
+                                                                              (SumType.inj_SumType ResourceRecordTypeTypes)
+                                                                              CNAME c_record  };
+                                       ret (Some c_record))).
+Proof.
+  intros.
+  destruct l as [ | ? [ | ?] ]; simpl in *; try discriminate.
+  pose proof (@refine_Singleton_Set _ q _ _ H); eauto.
+  - injection H0; intros; subst; simpl in H1; rewrite H1.
+    reflexivity.
+  - pose proof (@For_UnConstrQuery_In_Where_Prop DnsSchema Fin.F1 r_n _ _ _ H);
+      inversion H1; subst; eauto.
+Admitted.
+
+Lemma refine_Singleton_Set'
+  : forall (r_n : UnConstrQueryStructure DnsSchema) q bound l,
+    For (UnConstrQuery_In r_n Fin.F1
+                          (fun r : RawTuple =>
+                             Where (RDataTypeToRRecordType r!sRDATA <> CNAME /\ GetAttributeRaw r Fin.F1 = bound)
+                                   Return r )) ↝ l
+    -> refine
+         (SingletonSet (fun b : CNAME_Record =>      (* If the record is a CNAME, *)
+                          List.In (A := resourceRecord) b l
+                          /\ q <> QType_inj CNAME))
+         (ret None).
+Proof.
+Admitted.
+(*    MaxElements (fun r r' : resourceRecord => prefix (GetAttributeRaw r Fin.F1) (GetAttributeRaw r' Fin.F1))
+                For (Query_In r_o Fin.F1 (fun r : RawTuple => Where (prefix (GetAttributeRaw r Fin.F1) bound)
+                                                                    Return r )) ↝ l
+    -> Forall (fun r : resourceRecord => r!sNAME = bound) l
+    -> refine
+         (SingletonSet (fun b : CNAME_Record =>      (* If the record is a CNAME, *)
+                          List.In (A := resourceRecord) b l
+                          /\ q <> QType_inj CNAME))
+         (If q == (QType_inj CNAME) Then
+                                    (ret None)
+                                    Else
+         (Ifopt (hd_error l ) as record Then
+                                               (If (RDataTypeToRRecordType record!sRDATA) == CNAME Then
+                                               c_record <- {c_record : CNAME_Record | record =
+                                                                        @Tuple_DecomposeRawQueryStructure_inj'
+                                                                          _ DnsSchema Fin.F1 (Fin.FS (Fin.FS (Fin.FS (Fin.F1)))) _
+                                                                          (SumType.inj_SumType ResourceRecordTypeTypes)
+                                                                          CNAME c_record  };
+                   ret (Some c_record)
+                       Else ret None)
+                Else ret None)).
+Proof.
+  unfold refine, IfDec_Then_Else; intros.
+  destruct (q == CNAME); simpl in *; computes_to_inv; subst.
+  - computes_to_econstructor; split; intros.
+    discriminate.
+    intuition.
+  - destruct l; simpl in *; unfold SingletonSet.
+    + computes_to_inv; subst; computes_to_econstructor; split; intros.
+      discriminate.
+      intuition.
+    + match goal with
+        H : context[fin_eq_dec ?X ?Y] |- _ =>
+        destruct (fin_eq_dec X Y); simpl in H
+      end.
+      * computes_to_inv; subst.
+        destruct l; simpl in *.
+        { computes_to_econstructor; split; intros.
+          injections.
+          split; eauto; left.
+          destruct b as [? [? [? [? ?] ] ] ]; simpl in *.
+          unfold Tuple_DecomposeRawQueryStructure_inj'; simpl.
+          unfold icons2, ilist2_hd, ilist2_tl; simpl; repeat f_equal.
+          unfold SumType.inj_SumType; simpl.
+          unfold CNAME_Record2RRecord; simpl.
+          unfold VariantResourceRecord2RRecord; simpl.
+          unfold icons2; simpl.
+          repeat f_equal.
+          unfold Domain; simpl; reflexivity.
+          unfold Domain; simpl; reflexivity.
+          destruct prim_snd; destruct (@inil2 Type); reflexivity.
+          f_equal.
+          intuition.
+          destruct b as [? [? [? [? ?] ] ] ]; simpl in *.
+          unfold Tuple_DecomposeRawQueryStructure_inj' in *; simpl in *.
+          unfold icons2, ilist2_hd, ilist2_tl in *; simpl in *;
+            unfold SumType.inj_SumType in *; simpl in *.
+          unfold CNAME_Record2RRecord in *; simpl in *.
+          unfold VariantResourceRecord2RRecord in *; simpl in *.
+          unfold icons2 in *; simpl in *.
+          destruct v0 as [? [? [? [? ?] ] ] ]; simpl in *.
+          injections; simpl.
+          repeat f_equal.
+          destruct prim_snd; destruct (@inil2 Type); reflexivity.
+        }
+        admit.
+      * admit.
+Admitted. *)
+
+Lemma refine_If_Opt_Then_Else'
+  : forall (A B : Type) (c : option A) (x y : A -> Comp B),
+    (forall a, c = Some a -> refine (x a) (y a)) ->
+    forall x0 y0 : Comp B,
+      refine x0 y0 -> refine (Ifopt c as c' Then x c' Else x0) (Ifopt c as c' Then y c' Else y0).
+Proof.
+  intros; destruct c; simpl; eauto.
+Qed.
+
+Lemma refine_decides_QType_match
+  : forall rType qType,
+    ?[ QType_dec qType CNAME ] = true
+    -> refine {b : bool | decides b (QType_match rType qType)}
+              (ret (if (QType_dec rType CNAME) then true else false)).
+Proof.
+  intros ? ?; find_if_inside; intros; try discriminate.
+  subst.
+  refine pick val _; try reflexivity.
+  find_if_inside; subst; simpl.
+  econstructor 2; eauto.
+  intro; inversion H0; subst.
+  compute in H1; discriminate.
+  congruence.
+Qed.
+
+Lemma refine_If_Then_Bind {A B}
+  : forall b a (k : A -> Comp B) e,
+    refine (If b Then a' <- a; k a' Else e)
+           (a' <- a; If b Then k a' Else e).
+Proof.
+  destruct b; simpl; intros; try reflexivity.
+  intros ? ?.
+  computes_to_inv; eauto.
+Qed.
+
+Lemma refine_If_opt_hd_error_map {A B C}
+  : forall (f : A -> B) l t t' (e e' : Comp C),
+    (forall a , hd_error l = Some a -> refine (t (f a)) (t' a))
+    -> refine e e'
+    -> refine (Ifopt hd_error (map f l) as b' Then t b' Else e)
+              (Ifopt hd_error l as b' Then t' b' Else e').
+Proof.
+  destruct l; simpl; intros; subst; simpl; eauto.
+Qed.
+
+Lemma MaxElements_UnConstrQuery_In_Where_Prop {qs_schema}
+  : forall (idx : Fin.t (numRawQSschemaSchemas qs_schema))
+           (r_o0 : UnConstrQueryStructure qs_schema) (P : Ensemble RawTuple)
+           (l : list RawTuple) op,
+    DecideableEnsemble P ->
+    MaxElements op
+                (For (UnConstrQuery_In r_o0 idx (fun r0 : RawTuple => Where (P r0)
+                                                                            Return r0 ))) ↝ l -> Forall P l.
+Proof.
+Admitted.
+
+Definition QType_proj : QType -> option RRecordType. Admitted.
+
+Lemma refine_Process_Query_Exact_Match
+  : forall (r_o : UnConstrQueryStructure DnsSchema)
+           r_n e a1 qType a0 s,
+    DecomposeRawQueryStructureSchema_AbsR (qs_schema := DnsSchema) Fin.F1
+                                          (Fin.FS (Fin.FS (Fin.FS Fin.F1))) ResourceRecordTypeTypes
+                                          (SumType.SumType_index ResourceRecordTypeTypes)
+                                          (SumType.SumType_proj ResourceRecordTypeTypes)
+                                          (SumType.inj_SumType ResourceRecordTypeTypes) r_o r_n
+    -> refine
+         (a3 <- For (UnConstrQuery_In r_o Fin.F1
+                                      (fun r : RawTuple =>
+                                         Where (RDataTypeToRRecordType (GetAttributeRaw r (Fin.FS (Fin.FS (Fin.FS Fin.F1)))) <> CNAME
+                                                /\ GetAttributeRaw r Fin.F1 = a1)
+                                               Return r ));
+            a' <- ⟦element in a3
+                  | QType_match (RDataTypeToRRecordType (GetAttributeRaw element (Fin.FS (Fin.FS (Fin.FS Fin.F1)))))
+                                qType ⟧;
+            If negb (is_empty a3) Then ret (add_answers a' (buildempty true s a0))
+               Else e)
+         (If (QType_dec qType (EnumType.BoundedIndex_inj_EnumType ``("STAR"))) Then
+             (a3 <- For (UnConstrQuery_In r_o Fin.F1
+                                          (fun r : RawTuple =>
+                                             Where (RDataTypeToRRecordType (GetAttributeRaw r (Fin.FS (Fin.FS (Fin.FS Fin.F1)))) <> CNAME
+                                                    /\ GetAttributeRaw r Fin.F1 = a1)
+                                                   Return r ));
+                If negb (is_empty a3) Then ret (add_answers a3 (buildempty true s a0))
+                   Else e)
+             Else
+             (Ifopt QType_proj qType as rType Then
+                                              (a3 <- For (UnConstrQuery_In r_o Fin.F1
+                                                                           (fun r : RawTuple =>
+                                                                              Where (RDataTypeToRRecordType (GetAttributeRaw r (Fin.FS (Fin.FS (Fin.FS Fin.F1)))) = rType /\ RDataTypeToRRecordType (GetAttributeRaw r (Fin.FS (Fin.FS (Fin.FS Fin.F1)))) <> CNAME /\
+                                                                                     GetAttributeRaw r Fin.F1 = a1)
+                                                                                    Return r ));
+                                                 count <- Count (UnConstrQuery_In r_o Fin.F1
+                                                                                  (fun r : RawTuple =>
+                                                                                     Where (RDataTypeToRRecordType (GetAttributeRaw r (Fin.FS (Fin.FS (Fin.FS Fin.F1)))) <> rType
+                                                                                            /\ RDataTypeToRRecordType (GetAttributeRaw r (Fin.FS (Fin.FS (Fin.FS Fin.F1)))) <> CNAME
+                                                                                            /\ GetAttributeRaw r Fin.F1 = a1)
+                                                                                           Return r ));
+                                                 If negb (is_empty a3) || (le_lt_dec count 0) Then ret (add_answers a3 (buildempty true s a0))
+                                                    Else e)
+                                              Else e)).
+Admitted.
+
+Lemma refine_If_Else_Bind {A B}
+  : forall b a (k : A -> Comp B) t,
+    refine (If b Then t Else (a' <- a; k a'))
+           (a' <- a; If b Then t Else k a').
+Proof.
+  destruct b; simpl; intros; try reflexivity.
+  intros ? ?.
+  computes_to_inv; eauto.
+Qed.
+
+Arguments Iterate_Equiv_QueryResultComp_body : simpl never.
+
+Lemma refine_For_Bind {A B} :
+  forall (c : Comp (list A)) (f : A -> B),
+    refine (For (l <- c; ret (map f l)))
+           (l <- For c; ret (map f l)).
+Proof.
+  intros.
+  Local Transparent Query_For.
+  unfold Query_For; repeat rewrite refineEquiv_bind_bind.
+  simplify with monad laws.
+  f_equiv; intro.
+  intros ? ?; computes_to_inv; subst; computes_to_econstructor.
+  rewrite H; reflexivity.
+  Local Opaque Query_For.
+Qed.
+
+Lemma refine_MaxElements_map {A B}
+  : forall (f : A -> B) (c : Comp (list A)) (op : B -> B -> Prop),
+    refine (MaxElements op (l <- c; ret (map f l)))
+           (l <- MaxElements (fun a a' => op (f a) (f a')) c; ret (map f l)).
+Proof.
+  Local Transparent MaxElements.
+  intros; unfold MaxElements; simplify with monad laws.
+  rewrite refineEquiv_bind_bind; f_equiv; intro.
+  cut (forall a'',
+          refine {b : bool | decides b (UpperBound op (map f a) (f a''))}
+                 {b : bool | decides b (UpperBound (fun a0 a' : A => op (f a0) (f a')) a a'')}).
+  - generalize (UpperBound op (map f a)).
+    generalize (UpperBound (fun a0 a' : A => op (f a0) (f a')) a); intros.
+    induction a; simpl.
+    + rewrite refineEquiv_bind_unit; reflexivity.
+    + repeat setoid_rewrite refineEquiv_bind_bind.
+      rewrite IHa; simplify with monad laws.
+      f_equiv; intro.
+      setoid_rewrite H.
+      f_equiv; intro.
+      find_if_inside; rewrite refineEquiv_bind_unit; reflexivity.
+  - intros.
+    apply refineEquiv_pick_pick; intros.
+    apply decide_eq_iff_iff_morphism; eauto.
+    unfold UpperBound; split; intros;
+      induction a; simpl in *; intuition; subst; eauto.
+    Local Opaque MaxElements.
+Qed.
+
+Lemma refine_filter_Tuple_Decompose_inj' :
+  forall ns_results' : list NS_Record,
+    refine {ns_results : list NS_Record |
+            forall x : NS_Record,
+              List.In x ns_results <->
+              List.In x (A := resourceRecord)
+                      (map
+                         (Tuple_DecomposeRawQueryStructure_inj' (qs_schema := DnsSchema) Fin.F1
+                                                                (Fin.FS (Fin.FS (Fin.FS Fin.F1))) ResourceRecordTypeTypes
+                                                                (SumType.inj_SumType ResourceRecordTypeTypes) NS) ns_results')}
+           (ret ns_results').
+Proof.
+  intros; refine pick val _; eauto.
+  reflexivity.
+  induction ns_results'; simpl; split; intros; intuition eauto.
+  subst.
+  - left; destruct x as [? [? [? [? [ ] ] ] ] ]; reflexivity.
+  - right; apply IHns_results'; intuition eauto.
+  - left.
+    unfold NS_Record2RRecord, VariantResourceRecord2RRecord, Tuple_DecomposeRawQueryStructure_inj' in H0.
+    destruct x as [? [? [? [? [ ] ] ] ] ];
+      destruct a as [? [? [? [? [ ] ] ] ] ]; simpl in *.
+    unfold GetAttribute, GetAttributeRaw in *; simpl in *.
+    unfold icons2, ilist2_tl, ilist2_hd in H0; simpl in *.
+    injection H0; intros; subst.
+    reflexivity.
+  - right; apply IHns_results'; intuition eauto.
+Qed.
+
+Lemma refine_MaxElements' A op
+  : forall (ca ca' : Comp (list A)),
+    refine ca ca'
+    -> refine (MaxElements op ca) (MaxElements op ca').
+Proof.
+  simpl; intros.
+  Local Transparent MaxElements.
+  unfold MaxElements, refine; simpl in *; intros.
+  rewrite H; assumption.
+  Local Opaque MaxElements.
+Qed.
+
+Opaque Query_For.
+Opaque QueryResultComp.
+
 Lemma refine_If_Then_Else_true {C}
   : forall i (t e : Comp C),
     i = true
@@ -1146,4 +1877,80 @@ Lemma refine_If_Then_Else_false {C}
     -> refine (If i Then t Else e) e.
 Proof.
   intros; subst; simpl; reflexivity.
+Qed.
+
+Lemma refine_Process_Query_Imprecise_Match
+  : forall (r_o : QueryStructure DnsSchema)
+           (r_n : UnConstrQueryStructure DnsSchema)
+           bound p BStringId2 BStringId7,
+    DropQSConstraints_AbsR r_o r_n
+    -> refine
+         (a4 <- MaxElements (fun r r' : resourceRecord => prefix (GetAttributeRaw r Fin.F1) (GetAttributeRaw r' Fin.F1))
+             For (UnConstrQuery_In r_n Fin.F1
+                                   (fun r : RawTuple =>
+                                      Where (prefix (GetAttributeRaw r Fin.F1) bound /\ GetAttributeRaw r Fin.F1 <> bound)
+                                            Return r ));
+            a' <- {ns_results : list NS_Record | forall x : NS_Record, List.In x ns_results <-> List.In (A := resourceRecord) x a4};
+            If is_empty a4 Then ret (buildempty true BStringId2 p)
+               Else (a5 <- For (UnConstrQuery_In r_n Fin.F1
+                                                 (fun rRec : RawTuple =>
+                                                    Where (List.In (GetAttributeRaw rRec Fin.F1)
+                                                                   (map
+                                                                      (fun r : NS_Record => GetAttributeRaw r (Fin.FS (Fin.FS (Fin.FS Fin.F1))))
+                                                                      a'))
+                                                          Return rRec ));
+                       ret
+                         (add_additionals a5
+                                          (add_nses (map VariantResourceRecord2RRecord a') (buildempty true BStringId7 p)))))
+         (a4 <- MaxElements (fun r r' : resourceRecord => prefix (GetAttributeRaw r Fin.F1) (GetAttributeRaw r' Fin.F1))
+             For (UnConstrQuery_In r_n Fin.F1
+                                   (fun r : RawTuple =>
+                                      Where (RDataTypeToRRecordType r!sRDATA = NS /\ prefix (GetAttributeRaw r Fin.F1) bound)
+                                            Return r ));
+            a' <- {ns_results : list NS_Record | forall x : NS_Record, List.In x ns_results <-> List.In x (A := resourceRecord) a4};
+            If is_empty a' Then ret (buildempty true BStringId2 p)
+               Else (a5 <- For (UnConstrQuery_In r_n Fin.F1
+                                                 (fun rRec : RawTuple =>
+                                                    Where (List.In (GetAttributeRaw rRec Fin.F1)
+                                                                   (map
+                                                                      (fun r : NS_Record => GetAttributeRaw r (Fin.FS (Fin.FS (Fin.FS Fin.F1))))
+                                                                      a'))
+                                                          Return rRec ));
+                       ret
+                         (add_additionals a5
+                                          (add_nses (map VariantResourceRecord2RRecord a') (buildempty true BStringId7 p))))).
+Admitted.
+
+Lemma refine_decides_forall_and {A}
+  : forall (P Q : A -> Prop)
+           (P' Q' : @IndexedElement A -> Prop)
+           (R : @IndexedEnsemble A),
+    (forall a, P (indexedElement a) <-> P' a)
+    -> (forall a, Q (indexedElement a) <-> Q' a)
+    -> refine {b |
+               decides b
+                       (forall tup' : @IndexedElement A,
+                           R tup'
+                           -> Q' tup'
+                              /\ P' tup')}
+              (b' <- {b |
+                      decides b
+                              (forall tup' : @IndexedElement A,
+                                  R tup'
+                                  -> Q' tup')};
+                 If b' Then
+                    {b |
+                     decides b
+                             (forall tup' : @IndexedElement A,
+                                 R tup'
+                                 -> P' tup')}
+                    Else (ret false)).
+Proof.
+  unfold refine; intros; computes_to_inv; subst.
+  computes_to_econstructor.
+  find_if_inside; simpl in *; computes_to_inv; subst; simpl.
+  - destruct v; simpl in *; intros.
+    + intuition eauto.
+    + intro; eapply H1'; intros; eapply H2; eauto.
+  - intro; apply H1; intros; eapply H2; eauto.
 Qed.
